src/TLS.v
@@ -1,4 +1,4 @@
-Require Import List.
+Require Import List FunctionalExtensionality.
 Require String.
 Require Import Inhabit Foldable ClConv.
 Import ListNotations.
@@ -21,13 +21,14 @@ Parameter Session : Set.
 Parameter CipherID : Set.
 Parameter Version : Set.
 
+(*
 Record ClientHelloMsg :=
   {
     chSession : Session;
     chExtension : list ExtensionRaw;
     chCiphers : list CipherID
   }.
-
+*)
 Parameter serverGroups : list Group.
 
 Fixpoint findKeyShare ks gs :=
@@ -45,12 +46,82 @@ Definition intersect (xs ys : list Group) :=
 
 Parameter extension_KeyShare : list ExtensionRaw -> option (list KeyShare).
 Parameter extension_NegotiatedGroups : list ExtensionRaw -> list Group.
-Parameter word32 : Set.
-Parameter Handshake13 : Set.
-Parameter Packet13 : Set.
+Parameter Word32 : Set.
 Parameter PublicKey PrivateKey : Set.
 Parameter GroupPublic GroupKey : Set.
 Parameter Hash Cipher HashAndSignatureAlgorithm : Set.
+Parameter KeyUpdate : Set.
+Parameter Certificate CertificateChain : Set.
+Parameter Signature : Set.
+
+(*
+Definition CHandshake :=
+  ClientHelloMsg + ByteString.
+ *)
+
+Inductive CServerRandom := SR : ByteString -> CServerRandom.
+
+Inductive CHandshake :=
+| HClientHello : Version -> ByteString -> Session -> list ExtensionRaw -> list CipherID -> CHandshake
+| HServerHello : CServerRandom -> Session -> CipherID -> list ExtensionRaw -> CHandshake
+| HNewSessionTicket : Word32 -> Word32 -> ByteString -> ByteString -> list ExtensionRaw -> CHandshake
+| HEndOfEarlyData : CHandshake
+| HEncryptedExtensions : list ExtensionRaw -> CHandshake
+| HCertRequest : ByteString -> list ExtensionRaw -> CHandshake
+| HCertificate : ByteString -> CertificateChain -> list (list ExtensionRaw) -> CHandshake
+| HCertVerify : HashAndSignatureAlgorithm -> Signature -> CHandshake
+| HFinished : ByteString -> CHandshake
+| HKeyUpdate : KeyUpdate -> CHandshake.
+(*
+Definition  CPacket :=
+  list CHandshake + unit + ByteString.
+*)
+Inductive CPacket :=
+| PHandshake : list CHandshake -> CPacket
+| PChangeCipherSpec : CPacket
+| PAppData13 : ByteString -> CPacket.
+
+Record ClientHelloMsg :=
+  { chVersion : Version;
+    chRand : ByteString;
+    chSess : Session;
+    chExt : list ExtensionRaw;
+    chCipherIDs : list CipherID
+  }.
+                 
+Definition clientHello (h : CPacket) :=
+  match h with
+  | PHandshake [HClientHello v rand sess ext cipherIDs] =>
+    Some {| chVersion:=v; chRand:=rand; chSess:=sess; chExt:=ext; chCipherIDs:=cipherIDs  |}
+  | _ => None
+  end.
+
+Definition finished (h : CHandshake) :=
+  match h with
+  | HFinished bs => Some bs
+  | _ => None
+  end.
+
+Definition handshake (p : CPacket) :=
+  match p with
+  | PHandshake [h] => Some h
+  | _ => None
+  end.
+
+Definition changeCipherSpec (p : CPacket) :=
+  match p with
+  | PChangeCipherSpec => Some tt
+  | _ => None
+  end.
+
+Definition appData (p : CPacket) :=
+  match p with
+  | PAppData13 dat => Some dat
+  | _ => None
+  end.
+
+Parameter decodePacket : option (Hash * Cipher * ByteString * nat) -> ByteString -> option CPacket.
+
 
 (*
 Inductive eff_tls :=
@@ -64,152 +135,9 @@ Inductive eff_tls :=
 | makeCertVerify : PublicKey * PrivateKey * HashAndSignatureAlgorithm * ByteString -> eff_tls.
 *)
 
-Inductive eff_tls := recvClientHello | recvFinished | recvCCS | recvAppData | getRandomBytes | sendPacket | groupGetPubShared | makeCertVerify.
+Inductive eff_tls := recvData | getRandomBytes | sendPacket | groupGetPubShared | makeCertVerify.
 
-Definition args_tls ef :=
-  match ef with
-  | recvClientHello => unit
-  | recvFinished => option (Hash * Cipher * ByteString)
-  | recvCCS => unit
-  | recvAppData => option (Hash * Cipher * ByteString)
-  | getRandomBytes => nat
-  | sendPacket => Packet13 * option (Hash * Cipher * ByteString * nat)
-  | groupGetPubShared => GroupPublic
-  | makeCertVerify => PublicKey * PrivateKey * (HashAndSignatureAlgorithm) * ByteString
-  end.
-
-Definition rets_tls ef :=
-  match ef with
-  | recvClientHello => ClientHelloMsg * ByteString
-  | recvFinished => ByteString
-  | recvCCS => unit
-  | recvAppData => ByteString
-  | getRandomBytes => ByteString
-  | sendPacket => ByteString
-  | groupGetPubShared => option (GroupPublic * GroupKey)
-  | makeCertVerify => Handshake13
-  end.
-
-Definition lift_tls_core A (adef: A)(e : eff_tls)(a : rets_tls e -> A) e0
-  : rets_tls e0 -> A :=
-  match
-  e as e1
-  return ((rets_tls e1 -> A) -> rets_tls e0 -> A)
-  with
-  | recvClientHello =>
-    fun a0 : rets_tls recvClientHello -> A =>
-      match e0 as e1 return (rets_tls e1 -> A) with
-      | recvClientHello => a0
-      | _ => fun _ => adef
-      end
-  | recvFinished =>
-    fun a0 : rets_tls recvFinished -> A =>
-      match e0 as e1 return (rets_tls e1 -> A) with
-      | recvFinished => a0
-      | _ => fun _ => adef
-      end
-  | recvCCS =>
-    fun a0 : rets_tls recvCCS -> A =>
-      match e0 as e1 return (rets_tls e1 -> A) with
-      | recvCCS => a0
-      | _ => fun _ => adef
-      end
-  | recvAppData =>
-    fun a0 : rets_tls recvAppData -> A =>
-      match e0 as e1 return (rets_tls e1 -> A) with
-      | recvAppData => a0
-      | _ => fun _ => adef
-      end
-  | getRandomBytes =>
-    fun a0 : rets_tls getRandomBytes -> A =>
-      match e0 as e1 return (rets_tls e1 -> A) with
-      | getRandomBytes => a0
-      | _ => fun _ => adef
-      end
-  | sendPacket =>
-    fun a0 : rets_tls sendPacket -> A =>
-      match e0 as e1 return (rets_tls e1 -> A) with
-      | sendPacket => a0
-      | _ => fun _ => adef
-      end
-  | groupGetPubShared =>
-    fun a0 : rets_tls groupGetPubShared -> A =>
-      match e0 as e1 return (rets_tls e1 -> A) with
-      | groupGetPubShared => a0
-      | _ => fun _ => adef
-      end
-  | makeCertVerify =>
-    fun a0 : rets_tls makeCertVerify -> A =>
-      match e0 as e1 return (rets_tls e1 -> A) with
-      | makeCertVerify => a0
-      | _ => fun _ => adef
-      end
-  end a.
-
-Definition lift_tls A B(e : eff_tls)(a : rets_tls e -> A + option B) e0
-  : rets_tls e0 -> A + option B :=
-  match
-  e as e1
-  return ((rets_tls e1 -> A + option B) -> rets_tls e0 -> A + option B)
-  with
-  | recvClientHello =>
-    fun a0 : rets_tls recvClientHello -> A + option B =>
-      match e0 as e1 return (rets_tls e1 -> A + option B) with
-      | recvClientHello => a0
-      | _ => fun _ => inr None
-      end
-  | recvFinished =>
-    fun a0 : rets_tls recvFinished -> A + option B =>
-      match e0 as e1 return (rets_tls e1 -> A + option B) with
-      | recvFinished => a0
-      | _ => fun _ => inr None
-      end
-  | recvCCS =>
-    fun a0 : rets_tls recvCCS -> A + option B =>
-      match e0 as e1 return (rets_tls e1 -> A + option B) with
-      | recvCCS => a0
-      | _ => fun _ => inr None
-      end
-  | recvAppData =>
-    fun a0 : rets_tls recvAppData -> A + option B =>
-      match e0 as e1 return (rets_tls e1 -> A + option B) with
-      | recvAppData => a0
-      | _ => fun _ => inr None
-      end
-  | getRandomBytes =>
-    fun a0 : rets_tls getRandomBytes -> A + option B =>
-      match e0 as e1 return (rets_tls e1 -> A + option B) with
-      | getRandomBytes => a0
-      | _ => fun _ => inr None
-      end
-  | sendPacket =>
-    fun a0 : rets_tls sendPacket -> A + option B =>
-      match e0 as e1 return (rets_tls e1 -> A + option B) with
-      | sendPacket => a0
-      | _ => fun _ => inr None
-      end
-  | groupGetPubShared =>
-    fun a0 : rets_tls groupGetPubShared -> A + option B =>
-      match e0 as e1 return (rets_tls e1 -> A + option B) with
-      | groupGetPubShared => a0
-      | _ => fun _ => inr None
-      end
-  | makeCertVerify =>
-    fun a0 : rets_tls makeCertVerify -> A + option B =>
-      match e0 as e1 return (rets_tls e1 -> A + option B) with
-      | makeCertVerify => a0
-      | _ => fun _ => inr None
-      end
-  end a.
-
-Instance eff_tls_is_eff : is_eff eff_tls :=
-  { args := args_tls;
-    rets := rets_tls;
-    lift_eff := lift_tls }.
-
-Notation "r <- ef a ; p" :=
-  (@Eff eff_tls args_tls rets_tls _ ef a (fun r => p))
-    (at level 100, ef at level 0, right associativity).
+Parameter Packet13 Handshake13 : Set.
 
 Definition option_beq {A} (A_beq : A -> A -> bool) o1 o2 :=
   match o1, o2 with
@@ -238,24 +166,24 @@ Parameter extensionRaw_KeyShare : ByteString -> ExtensionRaw.
 Parameter extensionRaw_SupportedVersions : ByteString -> ExtensionRaw.
 Parameter handshake13 : list Handshake13 -> Packet13.
 Parameter serverHello13 : ByteString -> Session -> CipherID -> list ExtensionRaw -> Handshake13.
-Parameter changeCipherSpec : Packet13.
+(*Parameter changeCipherSpec : Packet13.*)
 Parameter extension_SignatureAlgorithms : list ExtensionRaw -> list (HashAndSignatureAlgorithm).
 
-Parameter Certificate CertificateChain : Set.
+
 Parameter getCertificates : CertificateChain -> list Certificate.
 Parameter defaultCertChain : PublicKey -> CertificateChain.
 Parameter certificate13 : ByteString -> CertificateChain -> list (list ExtensionRaw) -> Handshake13.
 Parameter empty : ByteString.
 Parameter ciphersuite_default : list Cipher.
-Parameter encodePacket13 : Packet13 -> ByteString.
 Parameter hashWith : Hash -> list ByteString -> ByteString.
 Parameter encryptedExtensions13 : list ExtensionRaw -> Handshake13.
 Parameter sniExt : ExtensionRaw.
 Parameter appData13 : ByteString -> Packet13.
+
 Parameter encodeEncryptedExt : list ExtensionRaw -> ByteString.
 Parameter CryptoError : Set.
 Parameter encodeGroupPublic : GroupPublic -> ByteString.
-Parameter decodeGroupPublic : Group -> ByteString -> CryptoError + GroupPublic.
+Parameter decodeGroupPublic : Group -> ByteString -> option GroupPublic.
 Parameter ba_convert : GroupKey -> ByteString.
 Parameter hashDigestSize : Hash -> nat.
 Parameter Word8 : Set.
@@ -356,270 +284,710 @@ Fixpoint replicate {A:Set} n (a:A) :=
   | S n' => a::replicate n' a
   end.
 
-Notation "r <- 'yield' e $ a ; p" :=
-  (Eff yield (existT e a)
-       (fun r' =>
-          match r' with
-          | existT e' x => lift_tls_core _ (Return tt) e (fun r => p) e' x
-          end))
+Definition args_tls' :=
+  nat + CPacket * option (Hash * Cipher * ByteString * nat) + GroupPublic + PublicKey * PrivateKey * HashAndSignatureAlgorithm * ByteString + unit + (unit + unit + unit + unit) * option (Hash * Cipher * ByteString * nat).
+
+
+Definition rets_tls' :=
+   option (GroupPublic * GroupKey) + CHandshake + ByteString + unit + ByteString * ClientHelloMsg.
+
+Notation "r <- 'yield' 'RecvClientHello' $ a ; p" :=
+  (Eff yield (inr (inr tt, a))
+       (fun r' => ((fun _ => Return tt) ||| (fun r => p)) r'))
+       (at level 100, right associativity).
+
+Notation "r <- 'yield' 'RecvData' $ a & o ; p" :=
+  (Eff yield (inl (inr a))
+       (fun r' => ((fun _ => Return o) ||| (fun r => p) ||| (fun _ => Return o) ||| (fun _ => Return o)) r'))
     (at level 100, right associativity).
 
-Instance sigT_rets_inhabit : Inhabit {e & rets_tls e} :=
-  { inhabitant := existT recvCCS tt }.
+Notation "r <- 'yield' 'RecvFinished' $ a ; p" :=
+  (Eff yield (inr (inl (inl (inr tt)), a))
+       (fun r' => ((fun _ => Return tt) ||| (fun r => p) ||| (fun _ => Return tt) ||| (fun _ => Return tt)) r'))
+    (at level 100, right associativity).
 
-Instance sigT_argss_inhabit : Inhabit {e & args_tls e} :=
-  { inhabitant := existT recvCCS tt }.
+Notation "r <- 'yield' 'RecvCCS' $ a ; p" :=
+  (Eff yield (inr (inl (inr tt), a))
+       (fun r' => ((fun _ => Return tt) ||| (fun r => p) |||(fun _ => Return tt)) r'))
+    (at level 100, right associativity).
 
-Definition doHandshake (cch: CertificateChain)(pr: PrivateKey)(_:{e & rets_tls e})
-  : t (const_yield { e & args_tls e }) (const_yield {e & rets_tls e}) unit :=
-  chr <- yield recvClientHello $ tt;
-  let certs := getCertificates cch in
-  let ch := fst chr in
-  let chEncoded := snd chr in
-  match chooseCipher (chCiphers ch) serverCiphers with
-  | None => Return tt
-  | Some cipher =>
-    let opt := extension_KeyShare ch.(chExtension) in
-    match opt with
-    | None => Return tt
-    | Some keyShares =>
-      let oks := findKeyShare keyShares serverGroups in
-      match oks with
-      | None => Return tt
-      | Some keyShare =>
-        let ecpub := decodeGroupPublic (ksGroup keyShare) (ksData keyShare) in
-        match ecpub with
-        | inl _ => Return tt
-        | inr cpub =>
-          mecdhePair <- yield groupGetPubShared $ cpub;
-          match mecdhePair with
-          | None => Return tt
-          | Some ecdhePair =>
-            let wspub := encodeGroupPublic (fst ecdhePair) in
-            let ecdhe := ba_convert (snd ecdhePair) in
-            let serverKeyShare := {| ksGroup := (ksGroup keyShare); ksData := wspub |} in
-            
-            (* sendServerHello *)
-            let ks := extensionEncode_KeyShare serverKeyShare in
-            let selectedVersion := extensionEncode_SupportedVersions TLS13 in
-            let extensions' :=
-                [ extensionRaw_KeyShare ks;
-                    extensionRaw_SupportedVersions selectedVersion ]
-            in
-            srand <- yield getRandomBytes $ 32;
-            shEncoded <- yield sendPacket $
-                      (handshake13 [serverHello13 srand (chSession ch) (cipherID cipher) extensions'], None);
-            let usedHash := cipherHash cipher in
-            let hCh := hashWith usedHash [chEncoded; shEncoded] in
-            let hsize := hashDigestSize usedHash in
-            let zero := b_replicate hsize w0 in
-            let earlySecret := hkdfExtract usedHash zero zero in
-            let clientEarlySecret := hkdfExpandLabel usedHash earlySecret (s2b "c e traffic") hCh hsize in
-            
-            let handshakeSecret := hkdfExtract usedHash (hkdfExpandLabel usedHash earlySecret (s2b "derived") (hashWith usedHash [s2b ""]) hsize) ecdhe in
-            let clientHandshakeSecret := hkdfExpandLabel usedHash handshakeSecret (s2b "c hs traffic") hCh hsize in
-            let serverHandshakeSecret := hkdfExpandLabel usedHash handshakeSecret (s2b "s hs traffic") hCh hsize in
-            ccsEncoded <- yield sendPacket $ (changeCipherSpec, None);
-            let _ := tt in
-            extEncoded <- yield sendPacket $
-                       (handshake13 [encryptedExtensions13 []], Some (usedHash, cipher, serverHandshakeSecret, 0));
+Notation "r <- 'yield' 'RecvAppData' $ a ; p" :=
+  (Eff yield (inr (inl (inl (inl tt)), a))
+       (fun r' => ((fun _ => Return tt) ||| (fun r => p) ||| (fun _ => Return tt) ||| (fun _ => Return tt)) r'))
+    (at level 100, right associativity).
 
-            let hashSigs := extension_SignatureAlgorithms ch.(chExtension) in
-            let mcred := decideCredInfo pr certs hashSigs in
-            match mcred with
-            | None => Return tt
-            | Some pubhs =>
-              let pub := fst pubhs in
-              let hashSig := snd pubhs in
-              certEncoded <- yield sendPacket $
-                          (handshake13 [certificate13 empty cch [[]]], Some (usedHash, cipher, serverHandshakeSecret, 1));
-              let hashed := hashWith (cipherHash cipher) [chEncoded; shEncoded; extEncoded; certEncoded] in
-              cv <- yield makeCertVerify $ (pub,pr,hashSig,hashed);
-              cvEncoded <- yield sendPacket $
-                        (handshake13 [cv], Some (usedHash, cipher, serverHandshakeSecret, 2));
-              let hashed' := hashWith (cipherHash cipher) [chEncoded; shEncoded; extEncoded; certEncoded; cvEncoded] in
-              finEncoded <- yield sendPacket $
-                         (handshake13 [finished13 (makeVerifyData usedHash serverHandshakeSecret hashed')],
-                          Some (usedHash, cipher, serverHandshakeSecret, 3));
+Notation "r <- 'yield' 'GetRandomBytes' $ a ; p" :=
+  (Eff yield (inl (inl (inl (inl (inl a)))))
+       (fun r' => ((fun _ => Return tt) ||| (fun r => p) ||| (fun _ => Return tt) ||| (fun _ => Return tt)) r'))
+    (at level 100, right associativity).
 
-              let hashed'' := hashWith (cipherHash cipher) [chEncoded; shEncoded; extEncoded; certEncoded; cvEncoded; finEncoded] in
-              let applicationSecret := hkdfExtract usedHash (hkdfExpandLabel usedHash handshakeSecret (s2b "derived") (hashWith usedHash [s2b ""]) hsize) zero in
-              let clientApplicationSecret := hkdfExpandLabel usedHash applicationSecret (s2b "c ap traffic") hashed'' hsize in
-              let serverApplicationSecret := hkdfExpandLabel usedHash applicationSecret (s2b "s ap traffic") hashed'' hsize in
+Notation "r <- 'yield' 'SendPacket' $ a ; p" :=
+  (Eff yield (inl (inl (inl (inl (inr a)))))
+       (fun r' => ((fun _ => Return tt) ||| (fun r => p) ||| (fun _ => Return tt)||| (fun _ => Return tt)) r'))
+    (at level 100, right associativity).
 
-              _ <- yield recvCCS $ tt;
-              fin <- yield recvFinished $ (Some (usedHash, cipher, clientHandshakeSecret));
-              if ByteString_beq fin (makeVerifyData usedHash clientHandshakeSecret hashed'') then
-                nat_rect_nondep
-                  (fun _ => Return tt)
-                  (fun _ rec _ =>
-                     data <- yield recvAppData $ (Some (usedHash, cipher, clientApplicationSecret));
-                       _ <- yield sendPacket $ (appData13 (mconcat ([s2b ("HTTP/1.1 200 OK" ++ CR ++ LF ++ "Content-Type: text/plain" ++ CR ++ LF ++ CR ++ LF ++ "Hello, "); data; s2b ("!" ++ CR ++ LF)] ++ replicate 1000 (s2b ".."))), Some (usedHash, cipher, serverApplicationSecret, 0));
-                     (rec tt))
-                  5 tt
-              else Return tt
+Notation "r <- 'yield' 'GroupGetPubShared' $ a ; p" :=
+  (Eff yield (inl (inl (inl (inr a))))
+       (fun r' => ((fun r => p) ||| (fun _ => Return tt) ||| (fun _ => Return tt) ||| (fun _ => Return tt) ||| (fun _ => Return tt)) r'))
+    (at level 100, right associativity).
+
+Notation "r <- 'yield' 'MakeCertVerify' $ a ; p" :=
+  (Eff yield (inl (inl (inr a)))
+       (fun r':rets_tls' => ((fun _ => Return tt) ||| (fun r => p) ||| (fun _ => Return tt) ||| (fun _ => Return tt) ||| (fun _ => Return tt)) r'))
+    (at level 100, right associativity).
+
+Instance sigT_rets_inhabit : Inhabit rets_tls' :=
+  { inhabitant := inl (inr tt) }.
+
+Instance sigT_argss_inhabit : Inhabit args_tls' :=
+  { inhabitant := inl (inr tt) }.
+
+Parameter ProtocolType : Set.
+Inductive Header := header : ProtocolType -> Version -> nat -> Header.
+
+Definition hdReadLen hd :=
+  match hd with
+  | header _ _ n => n
+  end.
+
+Parameter decodeHeader : ByteString -> Header.
+Parameter decodeRecord : Header -> option (Hash * Cipher * ByteString * nat) -> ByteString -> option CPacket.
+Parameter Bsplit :  ByteString -> nat -> ByteString * ByteString.
+
+Definition recvExactBytes bs0 n
+  : t (const_yield args_tls') (const_yield rets_tls') (option (ByteString * ByteString) ) := Eval unfold sum_merge in
+  nat_rect_nondep
+    (fun _ => Return None)
+    (fun _ rec accum =>
+       bs <- yield RecvData $ tt & None;
+       let bs' := mconcat [accum; bs] in
+       if Nat.ltb n (Blength bs') then
+         rec bs'
+       else
+         Return (Some (Bsplit bs' n)))
+    n bs0.
+
+Definition recvAndParse bs0 s o : t (const_yield args_tls') (const_yield rets_tls') (ByteString * option rets_tls') :=
+  hd <<- recvExactBytes bs0 5;
+  match hd with
+  | None => Return (bs0,None)
+  | Some p =>
+    let hd' := fst p in
+    let rem := snd p in
+    let header := decodeHeader hd' in
+    obs <<- recvExactBytes rem (hdReadLen header);
+    match obs with
+    | None => Return (rem,None)
+    | Some p =>
+      let bs := fst p in
+      let rem := snd p in
+      match decodeRecord header o bs with
+      | None => Return (rem,None)
+      | Some r =>
+        match s with
+        | inr tt =>
+          match clientHello r with
+          | None => Return (rem,None)
+          | Some c => Return (rem,Some (inr (bs,c)))
+          end
+        | inl (inr tt) =>
+          match changeCipherSpec r with
+          | None => Return (rem,None)
+          | Some tt => Return (rem,Some (inl (inr tt)))
+          end
+        | inl (inl (inr tt)) =>
+          match handshake r with
+          | None => Return (rem,None)
+          | Some h =>
+            match finished h with
+            | None => Return (rem,None)
+            | Some f => Return (rem,Some (inl (inl (inr f))))
             end
+          end
+        | inl (inl (inl tt)) =>
+          match appData r with
+          | None => Return (rem,None)
+          | Some a => Return (rem,Some (inl (inl (inr a))))
           end
         end
       end
     end
   end.
 
-Definition main_loop fuel :=
-  nat_rect_nondep
-    (fun _ => _)
-    (fun _ rec l =>
-       list_rec_nondep
-         (fun l0 => rec l0)
-         (fun c l' rec_inner l0n =>
-            let l0 := fst l0n in
-            let n := snd l0n in
-            o <- receive tt;
-              match o with
-              | None => rec_inner (l0, S n)
-              | Some r =>
-                a <- resume c $ r;
-                  _ <- ask a;
-                  rec_inner (replace_list n c l0, S n)
-              end)
-       o <- newAccept sock;
-         match o with
-         | Some s =>
-           pipe (doHandshake certs keys)
-                (fun cnew => 
+Notation "x <~ 'ifSome' o 'else' q ; p" :=
+  (option_branch (fun x => p) q o)
+    (at level 100, right associativity).
 
-Definition loop_ex (n i : nat) :=
-  let_coro c0 := ex_coroutine 0 in
-      nat_rect_nondep
-        (fun l =>
-           match nth_err _ l i : option (@coro_type nat nat _ _) with
-           | Some c =>
-             r <- resume c $ 1;
-               putN r;
-               Return _ _ (Some tt)
-           | None => Return args_effect rets_effect None
-           end)
-        (fun m rec l =>
-           putN (0:args_effect putNat);
-             pipe (ex_coroutine m : @coro_type nat nat _ _)
-                  (fun cm =>
-                     rec (cm::l)))
-        n [c0].
+Definition doHandshake (fuel:nat) (cch: CertificateChain)(pr: PrivateKey)(_: rets_tls')
+  : t (const_yield args_tls') (const_yield rets_tls') unit := Eval unfold option_branch in
+  let certs := getCertificates cch in
+  d' <- yield RecvClientHello $ None;
+  let chEncoded := fst d' in
+  let sess := chSess (snd d') in
+  let chExts := chExt (snd d') in
+  let cipherIDs := chCipherIDs (snd d') in
+  cipher <~ ifSome chooseCipher cipherIDs serverCiphers else Return tt;
+  keyShares <~ ifSome extension_KeyShare chExts else Return tt;
+  keyShare <~ ifSome findKeyShare keyShares serverGroups else Return tt;
+  cpub <~ ifSome decodeGroupPublic (ksGroup keyShare) (ksData keyShare) else Return tt;
+  mecdhePair <- yield GroupGetPubShared $ cpub;
+  ecdhePair <~ ifSome mecdhePair else Return tt;
+  let wspub := encodeGroupPublic (fst ecdhePair) in
+  let ecdhe := ba_convert (snd ecdhePair) in
+  let serverKeyShare := {| ksGroup := ksGroup keyShare; ksData := wspub |} in
+  
+  (* sendServerHello *)
+  let ks := extensionEncode_KeyShare serverKeyShare in
+  let selectedVersion := extensionEncode_SupportedVersions TLS13 in
+  let extensions' :=
+      [ extensionRaw_KeyShare ks;
+          extensionRaw_SupportedVersions selectedVersion ]
+  in
+  srand <- yield GetRandomBytes $ 32;
+  shEncoded <- yield SendPacket $
+            (PHandshake [HServerHello (SR srand) sess (cipherID cipher) extensions'], None);
+  let usedHash := cipherHash cipher in
+  let hCh := hashWith usedHash [chEncoded; shEncoded] in
+  let hsize := hashDigestSize usedHash in
+  let zero := b_replicate hsize w0 in
+  let earlySecret := hkdfExtract usedHash zero zero in
+  let clientEarlySecret := hkdfExpandLabel usedHash earlySecret (s2b "c e traffic") hCh hsize in
+  
+  let handshakeSecret := hkdfExtract usedHash (hkdfExpandLabel usedHash earlySecret (s2b "derived") (hashWith usedHash [s2b ""]) hsize) ecdhe in
+  let clientHandshakeSecret := hkdfExpandLabel usedHash handshakeSecret (s2b "c hs traffic") hCh hsize in
+  let serverHandshakeSecret := hkdfExpandLabel usedHash handshakeSecret (s2b "s hs traffic") hCh hsize in
+  ccsEncoded <- yield SendPacket $ (PChangeCipherSpec, None);
+  extEncoded <- yield SendPacket $
+             (PHandshake [HEncryptedExtensions []], Some (usedHash, cipher, serverHandshakeSecret, 0));
 
+  let hashSigs := extension_SignatureAlgorithms chExts in
+  pubhs <~ ifSome decideCredInfo pr certs hashSigs else Return tt;
+  let pub := fst pubhs in
+  let hashSig := snd pubhs in
+  certEncoded <- yield SendPacket $
+              (PHandshake [HCertificate empty cch [[]]], Some (usedHash, cipher, serverHandshakeSecret, 1));
+  let hashed := hashWith (cipherHash cipher) [chEncoded; shEncoded; extEncoded; certEncoded] in
+  cv <- yield MakeCertVerify $ (pub,pr,hashSig,hashed);
+  cvEncoded <- yield SendPacket $
+            (PHandshake [cv], Some (usedHash, cipher, serverHandshakeSecret, 2));
+  let hashed' := hashWith (cipherHash cipher) [chEncoded; shEncoded; extEncoded; certEncoded; cvEncoded] in
+  finEncoded <- yield SendPacket $
+             (PHandshake [HFinished (makeVerifyData usedHash serverHandshakeSecret hashed')],
+              Some (usedHash, cipher, serverHandshakeSecret, 3));
+
+  let hashed'' := hashWith (cipherHash cipher) [chEncoded; shEncoded; extEncoded; certEncoded; cvEncoded; finEncoded] in
+  let applicationSecret := hkdfExtract usedHash (hkdfExpandLabel usedHash handshakeSecret (s2b "derived") (hashWith usedHash [s2b ""]) hsize) zero in
+  let clientApplicationSecret := hkdfExpandLabel usedHash applicationSecret (s2b "c ap traffic") hashed'' hsize in
+  let serverApplicationSecret := hkdfExpandLabel usedHash applicationSecret (s2b "s ap traffic") hashed'' hsize in
+
+  _ <- yield RecvCCS $ None;
+  fin <- yield RecvFinished $ (Some (usedHash, cipher, clientHandshakeSecret, 0));
+  if ByteString_beq fin (makeVerifyData usedHash clientHandshakeSecret hashed'') then
+    nat_rect_nondep
+      (fun _ => Return tt)
+      (fun _ rec _ =>
+         data <- yield RecvAppData $ (Some (usedHash, cipher, clientApplicationSecret, 0));
+         x <- yield SendPacket $ (PAppData13 (mconcat ([s2b ("HTTP/1.1 200 OK" ++ CR ++ LF ++ "Content-Type: text/plain" ++ CR ++ LF ++ CR ++ LF ++ "Hello, "); data; s2b ("!" ++ CR ++ LF)])), Some (usedHash, cipher, serverApplicationSecret, 0));
+         rec tt)
+      fuel tt
+  else Return tt
+.
+
+Opaque replicate.
 
 Definition doHandshake_derive :
   { state & { step &
-              forall certs priv,
-                { init | @equiv_coro' _ _ _ _ _ state step init (doHandshake certs priv) }}}.
+              forall fuel certs priv,
+                { init | @equiv_coro' _ _ _ _ _ state step init (doHandshake fuel certs priv) }}}.
 Proof.
   do 3 eexists.
-  derive_coro (tt,certs,priv).
   unfold doHandshake.
-  derive' (tt, certs, priv).
-Defined.
+  Set Ltac Profiling.
+  derive_coro (tt,fuel,certs,priv).
+  Show Ltac Profile.
+  Time Defined.
 
-Definition doHandshake_step := Eval cbv [projT1 projT2 doHandshake doHandshake_derive] in (projT1 (projT2 doHandshake_derive)).
+Definition doHandshake_step := projT1 (projT2 doHandshake_derive).
+
+Definition doHandshake_equiv fuel certs keys :
+  equiv_coro' doHandshake_step _ (doHandshake fuel certs keys) :=
+  proj2_sig (projT2 (projT2 doHandshake_derive) fuel certs keys).
+
+Definition doHandshake_equiv' fuel certs keys
+  : equiv_coro' ltac:(let x := eval simpl in (projT1 (projT2 doHandshake_derive)) in exact x) ltac:(let x := eval simpl in (proj1_sig (projT2 (projT2 doHandshake_derive) fuel certs keys)) in exact x) (doHandshake fuel certs keys) :=
+  doHandshake_equiv fuel certs keys.
+
+Hint Resolve doHandshake_equiv doHandshake_equiv' : equivc.
+Hint  Resolve doHandshake_equiv : equivc'.
+    
+Definition readWrite fuel certs keys(_: rets_tls') : t (const_yield args_tls') (const_yield rets_tls') (option unit) :=
+  pipe (doHandshake fuel certs keys) (fun c : coro_type doHandshake_step =>
+  nat_rect_nondep
+    (fun _ => Return None)
+    (fun _ rec (bac: ByteString * rets_tls' * coro_type doHandshake_step) =>
+       let bs := fst (fst bac) in
+       let a := snd (fst bac) in
+       let c := snd bac in
+       r <- resume c $ a;
+         match r with
+         | inr eo =>
+           a' <<- recvAndParse bs (fst eo) (snd eo);
+           a'' <~ ifSome snd a' else Return None;
+           rec (fst a', a'', c)
+         | _ =>
+           a' <- yield r;
+           rec (bs, a', c)
+         end)
+    fuel (empty, inl (inr tt), c)).
+
+Inductive GenForall2_prod_r (A A1 A2 : Set)(R : A1 -> A2 -> Prop) : A * A1 -> A * A2 -> Prop :=
+  GenForall2_prod_r_rule : forall a x1 x2, R x1 x2 -> GenForall2_prod_r A A1 A2 R (a,x1) (a,x2).
+
+Program Instance prod_r_HasGenForall2 (A:Set) : HasGenForall2 (prod A) :=
+  { GenForall2 := GenForall2_prod_r A }.
+
+Program Instance id_HasGenForall2 : HasGenForall2 (fun A:Set => A) :=
+  { GenForall2 := fun A1 A2 R => R }.
+
+Instance ByteString_inhabitant : Inhabit ByteString :=
+  { inhabitant := empty }.
+
+Ltac derive_core'' ptr env :=
+  unfold recvExactBytes;
+  st_op_to_ev;[
+  lazymatch goal with
+    |- equiv' _ _ _ ?prog _ =>
+    lazymatch prog with
+    | @Eff _ ?args ?rets ?C ?e _ _ =>
+      lazymatch C with
+      | unit =>
+        let fv := free_var prog env in
+        eapply (Equiv'Eff (ptr (inl fv)) e);
+        [ let H := fresh in
+          intro H;
+          derive_core'' (fun x => ptr (inr x)) (fv,H)
+        | intros; dest_step]
+      | _ =>
+        eapply (Equiv'Eff (ptr (inl env)) e);
+        [ let H := fresh in
+          intro H;
+          derive_core'' (fun _x => ptr (inr _x)) (env,H)
+        | intros; dest_step]
+      end
+    | Return _ =>
+      idtac
+    | bind ?c _ =>
+(*      let c' := (eval red in c) in
+      change c with c';*)
+      let _s := next_state in
+      lazymatch _s with
+        (?stateF, ?ptr, ?stepF) =>
+        eapply (derive_bind _ (fun _ => _) (fun _ => _));
+          [ (* solve [repeat match goal with
+                            H : _ |- _ =>
+                            eapply (H stateF _ _ _ env _ _ _ ptr _ stepF);
+                            simpl; reflexivity
+                          end]
+            ||*)
+            let ptr := next_ptr open_constr:(fun _x => _x) in
+            derive_core'' ptr env
+          | let r := fresh in
+            intro r;
+            let _ := constr:(r) in
+            cbv beta;
+            let ptr := next_ptr open_constr:(fun _x => _x) in
+            derive_core'' ptr (env,r)
+          ]
+      end
+    | seqE' _ _ _ =>
+      eapply (derive_seqE' _ (fun s v => _) (fun s v => _) (fun s v => _));
+      [ let s := fresh in
+        let v := fresh in
+        intros s v;
+        derive_core'' ptr (env,s,v)
+      | let ptr := next_ptr open_constr:(fun _x => _x) in
+        derive_core'' ptr env ]
+    | (match ?x with inl _ => _ | inr _ => _ end) =>
+      eapply (derive_sum _ _ _ (fun a => _) (fun b => _) (fun a => _) (fun b => _));
+      [ let a := fresh in
+        intro a;
+        cbv beta;
+        let ptr := next_ptr open_constr:(fun _x => _x) in
+        derive_core'' ptr (env,a)
+      | let b := fresh in
+        intro b;
+        cbv beta;
+        let ptr := next_ptr open_constr:(fun _x => _x) in
+        derive_core'' ptr (env,b)
+      ]
+    | (match ?x with Some _ => _ | None => _ end) =>
+      eapply (derive_opt _ (fun _ => _) (fun _ => _) (fun _ => _));
+      [ let _a := fresh in
+        intro _a;
+        cbv beta;
+        let ptr := next_ptr open_constr:(fun _x => _x) in
+        derive_core'' ptr (env,_a)
+      | cbv beta;
+        let ptr := next_ptr open_constr:(fun _x => _x) in
+        derive_core'' ptr env
+      ]
+    | (match ?b with true => _ | false => _ end) =>
+      eapply derive_bool;
+      [ let ptr := next_ptr open_constr:(fun _x => _x) in
+        derive_core'' ptr env
+      | let ptr := next_ptr open_constr:(fun _x => _x) in
+        derive_core'' ptr env
+      ]
+    | nat_rect_nondep _ _ _ _ =>
+      idtac "test";
+      (solve [repeat match goal with
+                     | H : ?p |- _ => apply H
+                     end])
+      ||
+      (eapply (derive_nat_rect _ _ (fun a b => _) (fun a => _) (fun a => _));
+       [ let a := fresh in
+         intro a;
+         cbv beta;
+         let ptr := next_ptr open_constr:(fun _x => _x) in
+         derive_core'' ptr (env,a)
+       | let n := fresh in
+         let H := fresh in
+         let a := fresh in
+         intros n H a;
+         cbv beta;
+         let ptr := next_ptr open_constr:(fun _x => _x) in
+         derive_core'' ptr (env,n,a)
+      ])
+    | list_rec_nondep _ _ _ _ =>
+      (solve [repeat match goal with
+                   | H : ?p |- _ => apply H
+                   end])
+      ||
+      (eapply (derive_list_rec _ _ (fun _ _ => _) (fun _ => _) (fun _ => _));
+       [ let a := fresh in
+         intro a;
+         cbv beta;
+         let ptr := next_ptr open_constr:(fun _x => _x) in
+         derive_core'' ptr (env,a)
+       | let b := fresh in
+         let l := fresh in
+         let H := fresh in
+         let a := fresh in
+         intros b l H a;
+         cbv beta;
+         let ptr := next_ptr open_constr:(fun _x => _x) in
+         derive_core'' ptr (env,b,l,a)
+       ])
+    end
+  end|unify_fun..].
+
+Definition readWrite_derive :
+  { state & { step &
+              forall fuel certs priv,
+                { init | @equiv_coro _ _ _ state step init (readWrite fuel certs priv) } } }.
+Proof.
+  do 3 eexists.
+  lazymatch goal with
+    |- equiv_coro _ ?init ?x =>
+    let u := open_constr:(inl (tt,fuel,certs,priv)) in
+    unify init u
+  end;
+  econstructor.
+  econstructor.
+  intros.
+  split.
+  dest_step.
+  simpl.
+  assert (readWrite fuel certs priv r = ltac:(let x' := eval red in (readWrite fuel certs priv r) in
+                              let x'' := coro_to_state x' in exact x'')).
+  unfold readWrite, pipe.
+  lazymatch goal with
+  | |- @nat_rect_nondep ?A ?f0 _ ?k (?a1,?a2,?l) = nat_rect_nondep _ _ _ (_,_,?l') =>
+        lazymatch type of f0 with
+        | context [ @coro_type _ _ _ ?state ?step ] =>
+            cut
+             (GenForall2
+                (fun (coro : coro_type step) (st : state) =>
+                 equiv_coro' step st coro) l l');
+             [ generalize l, l', a1, a2;
+             induction k; intros;
+             lazymatch goal with
+             | |- nat_rect_nondep ?f ?f0 _ _ = nat_rect_nondep ?f' ?f0' _ _ =>
+                   let tmp := fresh in
+                   set (tmp := f);
+                    (let tmp' := fresh in
+                     set (tmp' := f');
+                      (let tmp0 := fresh in
+                       set (tmp0 := f0);
+                        (let tmp0' := fresh in
+                         set (tmp0' := f0'); simpl nat_rect_nondep; subst tmp;
+                          subst tmp'; subst tmp0; subst tmp0'; 
+                          cbv beta)))
+             | _ => idtac
+             end
+             | unfold GenForall2;
+                simpl; eauto with equivc ]
+        | ?T => idtac T
+        end
+  end.
+  mid_eq_core.
+  assert (equiv_coro'  doHandshake_step s t).
+  inversion H.
+  simpl. auto.
+  destruct H0.
+  inversion H0.
+  subst.
+  unfold  step_state at 1, seqE' at 1; rewrite H7.
+  specialize (H6 s0).
+  inversion H6.
+  unfold fst, snd in *.
+  rewrite <- H2.
+  subst.
+  unfold proc_coro at 1, seqE at 1.
+  rewrite <- H1.
+  destruct a.
+  repeat mid_eq_core.
+  apply IHfuel.
+  simpl.
+  unfold equiv_coro'.
+  eexists.
+  destruct e.
+  econstructor; eauto.
+  f_equal.
+  extensionality a'.
+  destruct (let (_,y) := a' in y).
+  apply IHfuel.
+  simpl.
+  eexists.
+  destruct e.
+  econstructor; eauto.
+  simpl.
+  reflexivity.
+  subst.
+  destruct H3.
+  unfold proc_coro at 1, seqE at 1.
+  unfold fst, snd.
+  rewrite H3.
+  rewrite <- H1.
+  reflexivity.
+
+  rewrite H.
+  clear H.
+  unfold step_state.
+
+  unfold recvAndParse, recvExactBytes.
+  (*
+  Set Ltac Debug.
+  derive_core'' open_constr:(fun a => inr a) (tt,fuel,certs,priv,r);
+  let ptr := next_ptr open_constr:(fun _x => _x) in
+  lazymatch goal with
+    |- equiv' ?step _ _ (Return ?r) _ =>
+    apply (Equiv'Return step _ (ptr r) None);
+      simpl;
+      split;
+      lazymatch goal with
+        |- _ ?x = _ =>
+        pattern_rhs x;
+          apply eq_refl
+      | _ => apply eq_refl
+      end
+  end.
+   *)
+Abort.
+
+Definition doHandshake_derive :
+  { state & { step &
+              forall fuel certs priv,
+                { init | @equiv_coro' _ _ _ _ _ state step init (doHandshake fuel certs priv) }}}.
+Proof.
+  do 3 eexists.
+  unfold doHandshake, recvClientHello, recvChangeCipherSpec, recvExactBytes.
+  derive_coro (tt,fuel,certs,priv).
+  unfold doHandshake, recvClientHello, recvAppData, recvHandshake, recvChangeCipherSpec, recvExactBytes.
+  unfold sum_merge.
+  lazymatch goal with
+    |- _ ?init _ =>
+    let u := open_constr:(inl (tt,fuel,certs,priv)) in
+    unify init u
+  end.
+  let r := fresh in
+  repeat eexists; try econstructor.
+  2: intros; dest_step.
+  intro r; derive_core open_constr:(fun x => inr x) ((tt,fuel,certs,priv),r).
+  all: try(
+  let ptr := next_ptr in
+  lazymatch goal with
+    |- equiv' ?step _ _ (Return ?r) _ =>
+    lazymatch type of r with
+    | unit => apply (Equiv'Return step _ (ptr r) None)
+    | _ => eapply (Equiv'Return step)
+    end
+  end;
+  split; simpl;
+  lazymatch goal with
+    |- _ ?a = _ =>
+    pattern_rhs a; apply eq_refl
+  | _ => apply eq_refl
+  end).
+  Grab Existential Variables.
+  all: exact unit.
+Defined.
 
 (*
-Definition doHandshake (cch: CertificateChain)(pr: PrivateKey) :=
-  chr <- recvClientHello tt;
-  let certs := getCertificates cch in
-  let ch := fst chr in
-  let chEncoded := snd chr in
-  match chooseCipher (chCiphers ch) serverCiphers with
-  | None => Return (Some "no cipher available")
-  | Some cipher =>
-    let opt := extension_KeyShare ch.(chExtension) in
-    match opt with
-    | None => Return (Some "no keyshare")
-    | Some keyShares =>
-      let oks := findKeyShare keyShares serverGroups in
-      match oks with
-      | None => Return (Some "no keyshare available")
-      | Some keyShare =>
-        let ecpub := decodeGroupPublic (ksGroup keyShare) (ksData keyShare) in
-        match ecpub with
-        | inl _ => Return (Some "no group")
-        | inr cpub =>
-          mecdhePair <- groupGetPubShared cpub;
-          match mecdhePair with
-          | None => Return (Some "generating ECDHE pair failed")
-          | Some ecdhePair =>
-            let wspub := encodeGroupPublic (fst ecdhePair) in
-            let ecdhe := ba_convert (snd ecdhePair) in
-            let serverKeyShare := {| ksGroup := (ksGroup keyShare); ksData := wspub |} in
-            
-            (* sendServerHello *)
-            let ks := extensionEncode_KeyShare serverKeyShare in
-            let selectedVersion := extensionEncode_SupportedVersions TLS13 in
-            let extensions' :=
-                [ extensionRaw_KeyShare ks;
-                    extensionRaw_SupportedVersions selectedVersion ]
-            in
-            srand <- getRandomBytes 32;
-            shEncoded <- sendPacket (handshake13 [serverHello13 srand (chSession ch) (cipherID cipher) extensions'], None);
-            let usedHash := cipherHash cipher in
-            let hCh := hashWith usedHash [chEncoded; shEncoded] in
-            let hsize := hashDigestSize usedHash in
-            let zero := b_replicate hsize w0 in
-            let earlySecret := hkdfExtract usedHash zero zero in
-            let clientEarlySecret := hkdfExpandLabel usedHash earlySecret (s2b "c e traffic") hCh hsize in
-            
-            let handshakeSecret := hkdfExtract usedHash (hkdfExpandLabel usedHash earlySecret (s2b "derived") (hashWith usedHash [s2b ""]) hsize) ecdhe in
-            let clientHandshakeSecret := hkdfExpandLabel usedHash handshakeSecret (s2b "c hs traffic") hCh hsize in
-            let serverHandshakeSecret := hkdfExpandLabel usedHash handshakeSecret (s2b "s hs traffic") hCh hsize in
-            ccsEncoded <- sendPacket (changeCipherSpec, None);
-            extEncoded <- sendPacket (handshake13 [encryptedExtensions13 []], Some (usedHash, cipher, serverHandshakeSecret, 0));
-
-            let hashSigs := extension_SignatureAlgorithms ch.(chExtension) in
-            let mcred := decideCredInfo pr certs hashSigs in
-            match mcred with
-            | None => Return None
-            | Some pubhs =>
-              let pub := fst pubhs in
-              let hashSig := snd pubhs in
-              certEncoded <- sendPacket (handshake13 [certificate13 empty cch [[]]], Some (usedHash, cipher, serverHandshakeSecret, 1));
-              let hashed := hashWith (cipherHash cipher) [chEncoded; shEncoded; extEncoded; certEncoded] in
-              cv <- makeCertVerify (pub,pr,hashSig,hashed);
-              cvEncoded <- sendPacket (handshake13 [cv], Some (usedHash, cipher, serverHandshakeSecret, 2));
-              let hashed' := hashWith (cipherHash cipher) [chEncoded; shEncoded; extEncoded; certEncoded; cvEncoded] in
-              finEncoded <- sendPacket (handshake13 [finished13 (makeVerifyData usedHash serverHandshakeSecret hashed')], Some (usedHash, cipher, serverHandshakeSecret, 3));
-
-              let hashed'' := hashWith (cipherHash cipher) [chEncoded; shEncoded; extEncoded; certEncoded; cvEncoded; finEncoded] in
-              let applicationSecret := hkdfExtract usedHash (hkdfExpandLabel usedHash handshakeSecret (s2b "derived") (hashWith usedHash [s2b ""]) hsize) zero in
-              let clientApplicationSecret := hkdfExpandLabel usedHash applicationSecret (s2b "c ap traffic") hashed'' hsize in
-              let serverApplicationSecret := hkdfExpandLabel usedHash applicationSecret (s2b "s ap traffic") hashed'' hsize in
-
-              _ <- recvCCS tt;
-              fin <- recvFinished (Some (usedHash, cipher, clientHandshakeSecret));
-              if ByteString_beq fin (makeVerifyData usedHash clientHandshakeSecret hashed'') then
-                nat_rect_nondep
-                  (fun _ => Return (Some "success"))
-                  (fun _ rec _ =>
-                     data <- recvAppData (Some (usedHash, cipher, clientApplicationSecret));
-                       _ <- sendPacket (appData13 (mconcat ([s2b ("HTTP/1.1 200 OK" ++ CR ++ LF ++ "Content-Type: text/plain" ++ CR ++ LF ++ CR ++ LF ++ "Hello, "); data; s2b ("!" ++ CR ++ LF)] ++ replicate 1000 (s2b ".."))), Some (usedHash, cipher, serverApplicationSecret, 0));
-                     (rec tt))
-                  5 tt
-              else Return None
-            end
-          end
-        end
-      end
+lazymatch goal with
+    |- equiv _ _ ?x =>
+    let y := eval red in x in
+        change x with y
+  | |- equiv_coro' _ _ ?x =>
+    let y := eval red in x in
+        change x with y
+  | _ => idtac
+  end;
+  simpl;
+  lazymatch goal with
+    |- _ ?init _ =>
+    let u := open_constr:(inl (tt,fuel,certs,priv)) in
+    unify init u
+  end;
+  let r := fresh in
+  repeat eexists; try econstructor;
+  [ intro r; derive_core open_constr:(fun x => inr x) ((tt,fuel,certs,priv),r)
+  | intros; dest_step'
+  ];
+  let ptr := next_ptr in
+  lazymatch goal with
+    |- equiv' _ _ (Return ?r) _ =>
+    eapply (Equiv'Return _ (ptr r));
+    simpl;
+    lazymatch goal with
+      |- _ ?a = _ =>
+      pattern_rhs a; apply eq_refl
+    | _ => apply eq_refl
     end
+  | _ => idtac
+  end.
+Time Defined.
+*)
+
+Inductive eff_conn := newAccept | perform | receive.
+
+
+Definition args_conn (e : eff_conn) :=
+  match e with
+  | newAccept => unit
+  | perform => string * args_tls'
+  | receive => unit
   end.
 
-Definition doHandshake_derive :
-  { state & { step &
-              forall certs priv,
-                { init | @equiv _ _ _ _ state step init (doHandshake certs priv) }}}.
+Definition rets_conn (e : eff_conn) :=
+  match e with
+  | newAccept => option string
+  | perform => unit
+  | receive => option (string * rets_tls')
+  end.
+
+Notation "r <- ef a ; p" :=
+  (@Eff eff_conn args_conn rets_conn _ ef a (fun r => p))
+    (at level 100, ef at level 0, right associativity).
+
+Definition doHandshake_step := projT1 (projT2 doHandshake_derive).
+
+
+Definition doHandshake_equiv fuel certs keys :
+  equiv_coro' doHandshake_step _ (doHandshake fuel certs keys) :=
+  proj2_sig (projT2 (projT2 doHandshake_derive) fuel certs keys).
+
+Definition doHandshake_equiv' fuel certs keys
+  : equiv_coro' ltac:(let x := eval simpl in (projT1 (projT2 doHandshake_derive)) in exact x) ltac:(let x := eval simpl in (proj1_sig (projT2 (projT2 doHandshake_derive) fuel certs keys)) in exact x) (doHandshake fuel certs keys) :=
+  doHandshake_equiv fuel certs keys.
+
+Hint Resolve doHandshake_equiv doHandshake_equiv' : equivc.
+Hint Resolve doHandshake_equiv : equivc'.
+
+Definition main_loop certs keys fuel :=
+  nat_rect_nondep
+    (fun _ => Return (Some tt))
+    (fun _ rec tr =>
+       osa <- newAccept tt;
+         match osa with
+         | Some sa =>
+           pipe (doHandshake 5 certs keys : coro_type doHandshake_step)
+                (fun c =>
+                   ef <- resume c $ inhabitant;
+                     _ <- perform (sa, ef);
+                     let tr' := insert sa c tr in
+                     rec tr')
+         | None =>
+           o <- receive tt;
+             match o with
+             | None => rec tr
+             | Some ar =>
+               let sa := fst ar in
+               let r := snd ar in
+               let ocoro := bsearch sa tr in
+               match ocoro with
+               | Some coro =>
+                 ef <- resume coro $ r;
+                   _ <- perform (sa, ef);
+                   let tr' := replace_map sa coro tr in
+                   rec tr'
+               | None => Return None
+               end
+             end
+         end)
+    fuel (Leaf _).
+
+Parameter certs_dummy : CertificateChain.
+Parameter privkey_dummy : PrivateKey.
+
+Instance CertificateChain_Inhabit : Inhabit CertificateChain :=
+  { inhabitant := certs_dummy }.
+
+Instance PrivateKey_Inhabit : Inhabit PrivateKey :=
+  { inhabitant := privkey_dummy }.
+
+Definition lift_conn A B(e : eff_conn)(a : rets_conn e -> A + option B) e0
+  : rets_conn e0 -> A + option B :=
+  match
+  e as e1
+  return ((rets_conn e1 -> A + option B) -> rets_conn e0 -> A + option B)
+  with
+  | newAccept =>
+    fun a0 : rets_conn newAccept -> A + option B =>
+      match e0 as e1 return (rets_conn e1 -> A + option B) with
+      | newAccept => a0
+      | _ => fun _ => inr None
+      end
+  | perform =>
+    fun a0 : rets_conn perform -> A + option B =>
+      match e0 as e1 return (rets_conn e1 -> A + option B) with
+      | perform => a0
+      | _ => fun _ => inr None
+      end
+  | receive =>
+    fun a0 : rets_conn receive -> A + option B =>
+      match e0 as e1 return (rets_conn e1 -> A + option B) with
+      | receive => a0
+      | _ => fun _ => inr None
+      end
+  end a.
+
+Instance eff_conn_is_eff : is_eff eff_conn :=
+  {| args := args_conn;
+    rets := rets_conn;
+    lift_eff := lift_conn |}.
+
+Definition main_loop_derive  :
+  { state & { step & forall certs keys fuel,
+                { init | @equiv _ _ _ _ state step init (main_loop certs keys fuel) }}}.
 Proof.
   do 3 eexists.
-  unfold doHandshake.
-  derive' (tt, certs, priv).
+  unshelve derive (tt,certs,keys,fuel); exact inhabitant.
 Defined.
 
-Definition doHandshake_step := Eval cbv [projT1 projT2 doHandshake doHandshake_derive] in (projT1 (projT2 doHandshake_derive)).
-*)
+
+Definition main_loop_step := Eval cbv [projT1 projT2 main_loop main_loop_derive] in (projT1 (projT2 (main_loop_derive))).
+
 Require Import extraction.ExtrHaskellString.
 
 Extract Inductive unit => "()" [ "()" ].
@@ -632,18 +1000,26 @@ Extract Inductive sum => "Prelude.Either" ["Prelude.Left" "Prelude.Right"].
 Extract Inductive option => "GHC.Base.Maybe" ["GHC.Base.Just" "GHC.Base.Nothing"].
 Extract Inductive Group => "T.Group" ["T.P256" "T.P384" "T.P521" "T.X25519"].
 Extract Inductive KeyShare => "I.KeyShareEntry" ["I.KeyShareEntry"].
+Extract Inductive CHandshake => "I.Handshake13" ["I.ClientHello13" "I.ServerHello13" "I.NewSessionTicket13" "I.EndOfEarlyData13" "I.EncryptedExtensions13" "I.CertRequest13" "I.Certificate13" "I.CertVerify13" "I.Finished13" "I.KeyUpdate13"].
+Extract Inductive CPacket => "I.Packet13" ["I.Handshake13" "I.ChangeCipherSpec13" "I.AppData13"].
+Extract Inductive Header => "I.Header" ["I.Header"].
+Extract Inductive CServerRandom => "I.ServerRandom" ["I.ServerRandom"].
+Extract Constant ProtocolType => "I.ProtocolType".
+Extract Constant decodeRecord => "Helper.decodeRecord".
+Extract Constant decodeHeader => "I.decodeHeader".
 Extract Constant Certificate => "X.Certificate".
 Extract Constant CertificateChain => "X.CertificateChain".
 Extract Constant getCertificates => "\cch -> case cch of { X.CertificateChain certs -> Prelude.map X.getCertificate certs }".
 Extract Constant HashAndSignatureAlgorithm => "I.HashAndSignatureAlgorithm".
 Extract Constant Group_eq_dec => "(GHC.Base.==)".
 Extract Constant Group_beq => "(GHC.Base.==)".
-Extract Constant Context => "T.Context".
 Extract Constant ExtensionRaw => "I.ExtensionRaw".
 Extract Constant Session => "I.Session".
 Extract Constant CipherID => "T.CipherID".
+(*
 Extract Constant Handshake13 => "I.Handshake13".
 Extract Constant Packet13 => "I.Packet13".
+*)
 Extract Constant ByteString => "B.ByteString".
 Extract Constant mconcat => "B.concat".
 Extract Constant extensionEncode_KeyShare => "(\ks -> I.extensionEncode (I.KeyShareServerHello ks))".
@@ -698,6 +1074,9 @@ Extract Constant appData13 => "I.AppData13".
 Extract Constant isDigitalSignaturePair => "I.isDigitalSignaturePair".
 Extract Constant signatureCompatible13 => "I.signatureCompatible13".
 Extract Constant certPubKey => "X.certPubKey".
+Extract Constant Word32 => "Data.Word.Word32".
+Extract Constant Signature => "I.Signature".
+Extract Constant KeyUpdate => "I.KeyUpdate".
 
 (*
 Extract Constant extension_KeyShare => "Helper.extension_KeyShare".
@@ -709,4 +1088,4 @@ Extract Inductive KeyShare => "Helper.KeyShare" ["Helper.Build_KeyShare"].
 Require Extraction.
 Extraction Language Haskell.
 
-Extraction "TLS.hs" doHandshake_step.
+Extraction "TLS.hs" main_loop_step.
